\documentclass{formation}
\title{Machine Learning}
\subtitle{Gradient de l'erreur}

\begin{document}

\maketitle

\begin{frame}
  \frametitle{Gradient et mise à jour}
  \begin{minipage}[l]{0.49\linewidth}
    \begin{center}
      $\boxed{y = a.x+b}$ \\
    \end{center}
    $E_{\Omega} = \frac{1}{2n}\sum_{i=[1..n]}( y_i^* - y_i )^2$ \\
    $E_{\Omega} = \frac{1}{2n}\sum_{i=[1..n]}( y_i^* - (a.x_i+b) )^2$ \\
    ... \\
    $\frac{\partial{E_{\Omega}}}{\partial{a}} = \frac{1}{n}\sum_{i=[1..n]}(a.x_i+b - y_i^*).x$ \\
    $\frac{\partial{E_{\Omega}}}{\partial{b}} = \frac{1}{n}\sum_{i=[1..n]}(a.x_i+b - y_i^*)$ \\
  \end{minipage}\hfill
  \begin{minipage}[c]{0.49\linewidth}
    $\;$ \\
    $\;$ \\
    $\;$ \\
    \begin{center}
      $\boxed{U^{2\;\prime}=2U\;'*U}$
    \end{center}
  \end{minipage}\hfill
  \begin{center}
    \textbf{M.A.J :} \\
    $\;$ \\
    $a \leftarrow a - \gamma.\frac{\partial{E_{\Omega}}}{\partial{a}}$ \\
    $b \leftarrow b - \gamma.\frac{\partial{E_{\Omega}}}{\partial{b}}$ \\
    $\;$ \\
    où $1 > \gamma > 0$ (learning rate)
  \end{center}
\end{frame}

\end{document}
%%% Local Variables:
%%% mode: latex
%%% TeX-master: t
%%% End:
